theories/tmc/sim/derived_rules.v
@@ -31,12 +31,8 @@ Section sim_GS.
   Qed.
 
   Lemma simv_call eₛ1 eₛ2 eₜ1 eₜ2 Φ :
-    ( ∀ func,
-      Func func ≈ Func func -∗
-      ⌜func ∈ dom progₛ ∧ func ∈ dom progₜ⌝
-    ) -∗
     ( ∀ func vₛ vₜ,
-      ⌜func ∈ dom progₛ ∧ func ∈ dom progₜ⌝ -∗
+      Func func ≈ Func func -∗
       vₛ ≈ vₜ -∗
       SIM progₛ; func vₛ ≳ progₜ; func vₜ [[ X ]] [[ Φ ]]
     ) -∗
@@ -44,12 +40,11 @@ Section sim_GS.
     SIM progₛ; eₛ2 ≳ progₜ; eₜ2 [[ X ]] [[ (≈) ]] -∗
     SIM progₛ; eₛ1 eₛ2 ≳ progₜ; eₜ1 eₜ2 [[ X ]] [[ Φ ]].
   Proof.
-    iIntros "#H Hsim Hsim1 Hsim2".
+    iIntros "Hsim Hsim1 Hsim2".
     simv_mono "Hsim2". iIntros "%vₛ2 %vₜ2 #Hv2".
     simv_mono "Hsim1". iIntros "%vₛ1 %vₜ1 #Hv1".
     destruct vₛ1, vₜ1; try iDestruct "Hv1" as %[]; try simv_strongly_stuck.
-    simv_apply ("Hsim" with "[] Hv2").
-    iApply ("H" $! func with "[//]").
+    simv_apply ("Hsim" with "[//] Hv2").
   Qed.
 
   Lemma simv_unop op eₛ eₜ Φ :
@@ -59,7 +54,8 @@ Section sim_GS.
   Proof.
     iIntros "Hsim HΦ".
     simv_mono "Hsim". iIntros "%vₛ %vₜ #Hv".
-    destruct op, vₛ, vₜ; try iDestruct "Hv" as %[]; try simv_strongly_stuck;
+    destruct vₛ, vₜ; try iDestruct "Hv" as %[];
+    destruct op; try simv_strongly_stuck;
       simv_pures;
       iApply "HΦ"; auto.
   Qed.
@@ -78,7 +74,7 @@ Section sim_GS.
     destruct op; try simv_strongly_stuck;
       simv_pures;
       iApply "HΦ"; auto.
-  Abort.
+  Qed.
 
   Lemma simv_if eₛ0 eₛ1 eₛ2 eₜ0 eₜ1 eₜ2 Φ :
     SIM progₛ; eₛ0 ≳ progₜ; eₜ0 [[ X ]] [[ (≈) ]] -∗
@@ -95,7 +91,7 @@ Section sim_GS.
   Lemma simv_constr constr eₛ1 eₛ2 eₜ1 eₜ2 Φ :
     SIM progₛ; eₛ1 ≳ progₜ; eₜ1 [[ X ]] [[ (≈) ]] -∗
     SIM progₛ; eₛ2 ≳ progₜ; eₜ2 [[ X ]] [[ (≈) ]] -∗
-    (∀ lₛ lₜ, lₛ ≈ lₜ -∗ Φ lₛ lₜ) -∗
+    (∀ lₛ lₜ, Loc lₛ ≈ Loc lₜ -∗ Φ lₛ lₜ) -∗
     SIM progₛ; &constr eₛ1 eₛ2 ≳ progₜ; &constr eₜ1 eₜ2 [[ X ]] [[ Φ ]].
   Proof.
     iIntros "Hsim1 Hsim2 HΦ".
@@ -104,13 +100,13 @@ Section sim_GS.
       [simv_constrₛ1 | simv_constrₛ2];
       simv_mono "Hsim1"; iIntros "%vₛ1 %vₜ1 #Hv1";
       simv_smart_mono "Hsim2"; iIntros "%vₛ2 %vₜ2 #Hv2";
-      simv_constr_det as lₛ lₜ "Hl" "Hl1" "Hl2";
+      simv_constr_det as lₛ lₜ "Hl";
       iApply "HΦ"; done.
   Qed.
   Lemma simv_constr_valₜ1 eₛ constr eₜ vₜ2 Φ :
     SIM progₛ; eₛ ≳ progₜ; eₜ [[ X ]] [[ (≈) ]] -∗
     ( ∀ vₛ l vₜ1,
-      l ↦ₜ constr -∗
+      (l +ₗ 0) ↦ₜ constr -∗
       (l +ₗ 1) ↦ₜ vₜ1 -∗
       (l +ₗ 2) ↦ₜ vₜ2 -∗
       vₛ ≈ vₜ1 -∗
@@ -121,13 +117,13 @@ Section sim_GS.
     iIntros "Hsim HΦ".
     simv_constrₜ;
       simv_smart_mono "Hsim"; iIntros "%vₛ %vₜ1 #Hv";
-      simv_constr_detₜ as l "Hl" "Hl1" "Hl2";
-      iApply ("HΦ" with "Hl Hl1 Hl2 Hv").
+      simv_constr_detₜ as l "Hl0" "Hl1" "Hl2";
+      iApply ("HΦ" with "Hl0 Hl1 Hl2 Hv").
   Qed.
   Lemma simv_constr_valₜ2 eₛ constr vₜ1 eₜ Φ :
     SIM progₛ; eₛ ≳ progₜ; eₜ [[ X ]] [[ (≈) ]] -∗
     ( ∀ vₛ l vₜ2,
-      l ↦ₜ constr -∗
+      (l +ₗ 0) ↦ₜ constr -∗
       (l +ₗ 1) ↦ₜ vₜ1 -∗
       (l +ₗ 2) ↦ₜ vₜ2 -∗
       vₛ ≈ vₜ2 -∗
@@ -138,32 +134,40 @@ Section sim_GS.
     iIntros "Hsim HΦ".
     simv_constrₜ;
       simv_smart_mono "Hsim"; iIntros "%vₛ %vₜ2 #Hv";
-      simv_constr_detₜ as l "Hl" "Hl1" "Hl2";
-      iApply ("HΦ" with "Hl Hl1 Hl2 Hv").
+      simv_constr_detₜ as l "Hl0" "Hl1" "Hl2";
+      iApply ("HΦ" with "Hl0 Hl1 Hl2 Hv").
   Qed.
 
-  Lemma simv_load eₛ eₜ Φ :
-    SIM progₛ; eₛ ≳ progₜ; eₜ [[ X ]] [[ (≈) ]] -∗
-    (∀ vₛ vₜ, vₛ ≈ vₜ -∗ Φ vₛ vₜ) -∗
-    SIM progₛ; !eₛ ≳ progₜ; !eₜ [[ X ]] [[ Φ ]].
-  Proof.
-    iIntros "Hsim HΦ".
-    simv_mono "Hsim". iIntros "%vₛ %vₜ #Hv".
-    destruct vₛ, vₜ; try iDestruct "Hv" as %[]; try simv_strongly_stuck.
-    simv_load as wₛ wₜ "Hw".
-    iApply ("HΦ" with "Hw").
-  Qed.
-
-  Lemma simv_store eₛ1 eₛ2 eₜ1 eₜ2 Φ :
+  Lemma simv_load eₛ1 eₛ2 eₜ1 eₜ2 Φ :
     SIM progₛ; eₛ1 ≳ progₜ; eₜ1 [[ X ]] [[ (≈) ]] -∗
     SIM progₛ; eₛ2 ≳ progₜ; eₜ2 [[ X ]] [[ (≈) ]] -∗
-    Φ ()%V ()%V -∗
-    SIM progₛ; eₛ1 <- eₛ2 ≳ progₜ; eₜ1 <- eₜ2 [[ X ]] [[ Φ ]].
+    (∀ vₛ vₜ, vₛ ≈ vₜ -∗ Φ vₛ vₜ) -∗
+    SIM progₛ; ![eₛ2] eₛ1 ≳ progₜ; ![eₜ2] eₜ1 [[ X ]] [[ Φ ]].
   Proof.
     iIntros "Hsim1 Hsim2 HΦ".
     simv_mono "Hsim2". iIntros "%vₛ2 %vₜ2 #Hv2".
     simv_mono "Hsim1". iIntros "%vₛ1 %vₜ1 #Hv1".
-    destruct vₛ1, vₜ1; try iDestruct "Hv1" as %[]; try simv_strongly_stuck.
+    destruct vₛ1, vₜ1; try iDestruct "Hv1" as %[];
+    destruct vₛ2, vₜ2; try iDestruct "Hv2" as %[];
+      try simv_strongly_stuck.
+    simv_load as wₛ wₜ "Hw".
+    iApply ("HΦ" with "Hw").
+  Qed.
+
+  Lemma simv_store eₛ1 eₛ2 eₛ3 eₜ1 eₜ2 eₜ3 Φ :
+    SIM progₛ; eₛ1 ≳ progₜ; eₜ1 [[ X ]] [[ (≈) ]] -∗
+    SIM progₛ; eₛ2 ≳ progₜ; eₜ2 [[ X ]] [[ (≈) ]] -∗
+    SIM progₛ; eₛ3 ≳ progₜ; eₜ3 [[ X ]] [[ (≈) ]] -∗
+    Φ ()%V ()%V -∗
+    SIM progₛ; eₛ1 <-[eₛ2]- eₛ3 ≳ progₜ; eₜ1 <-[eₜ2]- eₜ3 [[ X ]] [[ Φ ]].
+  Proof.
+    iIntros "Hsim1 Hsim2 Hsim3 HΦ".
+    simv_mono "Hsim3". iIntros "%vₛ3 %vₜ3 #Hv3".
+    simv_mono "Hsim2". iIntros "%vₛ2 %vₜ2 #Hv2".
+    simv_mono "Hsim1". iIntros "%vₛ1 %vₜ1 #Hv1".
+    destruct vₛ1, vₜ1; try iDestruct "Hv1" as %[];
+    destruct vₛ2, vₜ2; try iDestruct "Hv2" as %[];
+      try simv_strongly_stuck.
     simv_store.
   Qed.
 End sim_GS.
